ulib/experimental/Steel.ST.Effect.Atomic.fsti
@@ -75,6 +75,9 @@ effect STAtomicU (a:Type)
 (* Composing SteelAtomic and Pure computations *)
 polymonadic_bind (PURE, STAtomicBase) |> STAtomicBase = STAG.bind_pure_stag
 
+effect STAtomicBaseT (a:Type) (opened:inames) (obs:observability) (pre:pre_t) (post:post_t a) =
+  STAtomicBase a false opened obs pre post True (fun _ -> True)
+
 /// A version of the SteelAtomic effect with trivial requires and ensures clauses
 effect STAtomicT (a:Type) (opened:inames) (pre:pre_t) (post:post_t a) =
   STAtomic a opened pre post True (fun _ -> True)
